Sentences of the form "If P, then Q" are the most important kinds of propositions in mathematics.
# Definitions - Conditional Sentence
For propositions $P$ and $Q$, the **conditional sentenc** $P\implies Q$, is the proposotion "If $P$, then $Q$." Proposition $P$ is called the **antecedent** and $Q$ is the **consequent**. The sentence $P\implies Q$ is true if and only if $P$ is false or $Q$ is true.
The truth table for $P\implies Q$ is

## $P\implies Q$ Truth table

| $P$ | $Q$ | $P\implies Q$ |
| --- | --- | ------------- |
| F   | F   | T             |
| F   | T   | T             |
| T   | F   | F             |
| T   | T   | T             |

The only case where $P\implies Q$ is a false statement occurs on line 3 of its [[1.2 Conditionals and Biconditionals#$P implies Q$ Truth table|truth table]], when $P$ is true and $Q$ is false. This agrees with the way we understand promises.

# Example - Suppose someone makes this promise to a friend:
	"If the weather is warm, we will go hiking."
The ==antecedent== is "The weather is warm" and the ==consequent== is "We will go hiking." This promise would be broken if the weather turned out to be warm and the friends did *not* go hiking (line 3 of the [[1.2 Conditionals and Biconditionals#$P implies Q$ Truth table|truth table]]) . In every other situation, the statement is true:
- When the weather was warm and the friends went hiking (line 4 of the [[1.2 Conditionals and Biconditionals#$P implies Q$ Truth table|truth table]])
- Whether the friends go hiking or not, in the event that the weather is *not* warm, we wouldn't say the promise was broken. (These are lines 1 and 2 of the [[1.2 Conditionals and Biconditionals#$P implies Q$ Truth table|truth table]])
Our truth table definitions for $P\implies Q$ captures the same meaning for "If..., then..." that you have always used in mathematics.

# Example - if we think of x as some fixed real number, we all know that
	"If x>8, then x>5"
is a true statement, no matter what number $x$ we have in mind. Let's examine why we say this sentence is true for some specific values of $x$, where the antecedent $P$ is "$x>5$" and the consequent $Q$ is "$x>5$".
- When $x$ is a number greater than both 8 and 5 (for example, 11), both $P$ and $Q$ are true (as in line 4 of the [[1.2 Conditionals and Biconditionals#$P implies Q$ Truth table|truth table]]).
- When $x$ is between 5 and 8 (for example, 7), $P$ is false and $Q$ is true (as in line 2 of the [[1.2 Conditionals and Biconditionals#$P implies Q$ Truth table|truth table]]). 
- When $x$ is less than both 8 and 5 (for example, 2), we have the situation where $P=F$ and $Q=F$, (as in line 1 of the [[1.2 Conditionals and Biconditionals#$P implies Q$ Truth table|truth table]] ).
In all three, cases $P\implies Q$ is true. In fact, "If $x>8$", then $x>5$" is always true because there can be no case corresponding to an $x$ being greater than 8 and not being greater than 5.
We are not claiming that either $P$ or $Q$ is true. What we do say is that no matter what number we think of,
- *if* it is larger than 8, *then* it is also larger than 5.

One curious consequence of the truth table for $P\implies Q$ is that a conditional sentence may be true even when there is no connection between the antecedent and the consequent.
 The reason for this is that the truth value of $P\implies Q$ depends *only* on the truth value of components $P$ and $Q$, not on their interpretation. For this reason, all of the following are true:
- "If sin($\pi$) = 1, then 6 is prime." (line 1 of the [[1.2 Conditionals and Biconditionals#$P implies Q$ Truth table|truth table]])
- "$13>7\implies 2+3=5$." (line 4 of the [[1.2 Conditionals and Biconditionals#$P implies Q$ Truth table|truth table]])
- "$\pi=3\implies$ Paris is the capital of France." (line 2 of the [[1.2 Conditionals and Biconditionals#$P implies Q$ Truth table|truth table]])
and both of these are false by line 3 of the [[1.2 Conditionals and Biconditionals#$P implies Q$ Truth table|truth table]]:
- "If Saturn has rings, then $(2 + 3)^2=2^2+3^2$."
- "If $4\pi>10$", then 1 is a prime number."
Other consequences of the truth table for $P\implies Q$ are worth noting.
- When $P$ is false (lines 2 and 4), it doesn't matter what truth value $Q$ has: $P\implies Q$ will be true.
- When $Q$ is true (lines 1 and 2), it doesn't matter what truth value $P$ has: $P\implies Q$ will be true.
- When $P$ and $P\implies Q$ are both true (on line 1), $Q$ must also be true.
	Two propositions associated with $P\implies Q$ are its converse and contrapositive.

# Definition Let $P$ and $Q$ be proposition.
The **converse** of $P\implies Q$ is $Q\implies P$.
The **contrapositive** of $P\implies Q$ is $(\sim{Q})\implies(\sim{P})$.

For the conditional sentence "If $\pi$ is an integer, then 14 is even".
- The ==converse== of the sentence is "If 14 is even, then $\pi$ is an integer".
- The ==contrapositive== of the sentence is "If 14 is not even, then $\pi$ is not an integer."
 The sentence and its contrapositive are true, but the converse is false. The sentence and its contrapositive are true, but the converse is false.

For the sentence "If $1+1=2$, then $\sqrt{10}>3$".
- The ==converse== of the sentence is "If $\sqrt{10}>3$, then $1+1=2$."
- The ==contrapositive== of the sentence is "If $\sqrt{10}$ is not greater than 3, then $1+1$ is not equal to 2."
In this example, all three sentences are true.
	These two examples show that a *conditional sentence and its converse are not always equivalent*. Thus, the truth value of $P\implies Q$ *cannot* be inferred from its converse $Q\implies P$. However, a statement and its contrapositive are equivalent, as the following theorem shows.
# Theorem 1.2.1 For propositions $P$ and $Q$, $P\implies Q$ is equivalent to its contrapositive $(\sim{Q})\implies(\sim{P})$.
## Theorem 1.2.1 Proof:
	The proof is carried out by examination of the truth table.

| $P$ | $Q$ | $P\implies Q$ | $\sim{P}$ | $\sim{Q}$ | $(\sim{Q})\implies(\sim{P})$ |
| :-: | :-: | :-----------: | :-------: | :-------: | :--------------------------: |
|  T  |  T  |       T       |     F     |     F     |              T               |
|  F  |  T  |       T       |     T     |     F     |              T               |
|  T  |  F  |       F       |     F     |     T     |              F               |
|  F  |  F  |       T       |     T     |     T     |              T               |
$P\implies Q$ is equivalent to $(\sim{Q})\implies(\sim{P})$ because the third column in the truth table is identical to the sixth column.

# Biconditional Connective
The biconditional connective, defined next, is symbolized with a double arrow $\Leftarrow\Rightarrow$, which reminds one of both $\Leftarrow$ and $\Rightarrow$. This is no accident because $P\Leftarrow\Rightarrow Q$ is equivalent to $(P\implies Q)\land(Q\implies P)$.

# Definition - Biconditional
For propositions $P$ and $Q$, the **biconditional sentence** $P\Leftarrow\Rightarrow Q$ is the proposition "P if and only if Q". The sentence $P\Leftarrow\Rightarrow Q$ is true exactly when $P$ and $Q$ have the same truth values
- Mathematicians often abbreviate "$P$ if and only if $Q$" as "$P$ iff $Q$". The truth table for $P\Leftarrow\Rightarrow Q$ is

|  P  |  Q  | $P\Leftarrow\Rightarrow Q$ |
| :-: | :-: | :------------------------: |
|  F  |  F  |             T              |
|  F  |  T  |             F              |
|  T  |  F  |             F              |
|  T  |  T  |             T              |

# Theorem 1.2.2
For propositions $P$, $Q$, and $R$, the following are equivalent:

|         (a) $P\implies Q$          | and | $\sim{P}\lor Q$                         |
| :--------------------------------: | --- | --------------------------------------- |
|   (b) $P\Leftarrow\Rightarrow Q$   | and | $(P\implies Q)\land(Q\implies P)$       |
|     (c) $\sim{P\Rightarrow Q}$     | and | $P~\land\sim{Q}$                        |
|       (d) $\sim{(P\land Q)}$       | and | $P\Rightarrow\sim{Q}$                   |
|       (e) $\sim{(P\land Q)}$       | and | $Q\Rightarrow\sim{P}$                   |
| (f) $P\Rightarrow(Q\Rightarrow R)$ | and | $(P\land Q)\Rightarrow R$               |
|    (g) $P\Rightarrow(Q\land R)$    | and | $(P\Rightarrow Q)\land(P\Rightarrow R)$ |
|    (h) $(P\lor Q)\Rightarrow R$    | and | $(P\Rightarrow R)\land(Q\Rightarrow R)$ |
